progress

soundness.v
@@ -4,6 +4,27 @@ Require Import category.
 Require Import stlc.
 Require Import model.
 
+Fixpoint rename_denot {C} `{CartesianClosed C}
+{Γ Δ : context} (ρ : ∀ t, contains Γ t → contains Δ t) {struct Γ}:
+Hom (ctx_denot Δ) (ctx_denot Γ).
+Proof.
+  destruct Γ.
+  + refine terminal_map.
+  + simpl.
+    apply f_prod.
+    2:{
+      apply tm_denot.
+      apply var_term.
+      apply ρ.
+      apply var_zero.
+    }
+    - apply rename_denot.
+      intros.
+      apply ρ.
+      apply var_succ.
+      assumption.
+Defined.
+
 Fixpoint subst_denot {C} `{CartesianClosed C}
 {Γ Δ : context} (ρ : ∀ t, contains Γ t → term Δ t) {struct Γ}:
 Hom (ctx_denot Δ) (ctx_denot Γ).
@@ -23,6 +44,73 @@ Proof.
       apply var_succ.
       assumption.
 Defined.
+
+Lemma subst_rename
+{C} `{CartesianClosed C}
+{Γ}
+{Δ Ω : context}
+(var_to_var : ∀ t, contains Γ t → contains Δ t)
+(var_to_term : ∀ t, contains Δ t → term Ω t)
+(* {struct Γ} *)
+ :
+subst_denot (fun _ var => var_to_term _ (var_to_var _ var))
+= compose (rename_denot var_to_var) (subst_denot var_to_term).
+Proof.
+  induction Γ.
+  + simpl. 
+    apply terminal_uniq.
+  + simpl.
+    rewrite IHΓ.
+    symmetry.
+    apply f_prod_uniq.
+    - rewrite <- compose_assoc.
+      rewrite f_prod_comm1.
+      reflexivity.
+    - rewrite <- compose_assoc.
+      rewrite f_prod_comm2.
+Admitted.
+
+Lemma var_succ_denot :
+∀ {C} `{CartesianClosed C}
+{Γ t},
+@subst_denot _ _ _ _ _ _ Γ (context_cons t Γ) (fun _ x => (var_term (var_succ x))) = fst.
+Proof.
+  intros.
+  induction Γ.
+  + simpl.
+    apply terminal_uniq.
+  + simpl.
+    symmetry.
+    apply f_prod_uniq.
+    2:{ reflexivity. }
+    rewrite subst_rename with (var_to_term := fun _ x => var_term (var_succ x)).
+    f_equal.
+    - generalize Γ.
+      induction Γ0.
+      * simpl. apply terminal_uniq.
+Admitted.
+
+Lemma subst1_map_denot :
+∀ {C} `{CartesianClosed C}
+{Γ t}
+(e : term Γ t),
+subst_denot (subst1_map e) = f_prod (id _) (tm_denot e).
+Proof.
+  intros.
+  induction Γ.
+  + simpl.
+    rewrite terminal_obj_map.
+    reflexivity.
+  + simpl.
+    f_equal.
+    rewrite var_succ_denot.
+    symmetry.
+    apply f_prod_uniq.
+    - rewrite compose_id_r.
+      reflexivity.
+    - rewrite compose_id_r.
+      reflexivity.
+Qed.
 
 Definition ext_ctx_denot
 {C} `{CartesianClosed C}
@@ -121,7 +209,8 @@ Proof.
   + unfold app.
     simpl.
     rewrite subst_denot_decomp.
-   admit.
+    rewrite subst1_map_denot.
+    apply curry_prop.
   + simpl.
     unfold shift_one.
     rewrite subst_denot_decomp.
